experiments/003_malloc_ir/SirLean/Source/Spec.lean
@@ -11,20 +11,43 @@ instance (ranges : OccupiedMemory) (r : MemoryRange) : Decidable (ranges.Fresh r
   unfold OccupiedMemory.Fresh
   infer_instance
 
+theorem OccupiedMemory.empty_WF : OccupiedMemory.WF #[] := by simp [WF]
+
+theorem Allocator.sound_ensures_WF_occupied :
+    ∀ allocator : Allocator, allocator.Sound →
+    ∀ ranges : OccupiedMemory,
+    allocator.Provenance ranges → ranges.WF := by
+  intro allocator sound ranges provenance
+  simp [OccupiedMemory.WF]
+  cases provenance with
+  | empty => sorry
+  | alloc h => by
+    sorry
+
+
+
+
 
 def Allocator.bump : Allocator :=
-  fun occupied size => do
-    if occupied.isEmpty then
-      return 0
-    let r ← occupied.find? (fun r =>
-      let start := r.endExclusive
-      let r' := { addr := .ofNat start, size := size }
-      start ≤ UInt32.size ∧ size.toNat ≤ UInt32.size - start ∧ decide (occupied.Fresh r')
-    )
-    return r.addr
+  fun occupied size =>
+    let r := occupied.back?.getD ⟨0, 0⟩
+    let new_start := r.endExclusive
+    if new_start + size.toNat ≤ Word.size then
+      .some (.ofNat new_start)
+    else
+      .none
 
-
-theorem Allocator.bump_sound : Allocator.Sound Allocator.bump := by
-  sorry
+-- theorem Allocator.bump_sound : Allocator.Sound Allocator.bump := by
+--   intro ranges size addr _ h
+--   unfold Allocator.bump at h
+--   split at h
+--   · simp [OccupiedMemory.Fresh, MemoryRange.Disjoint]
+--
+--
+--
+--   · cases hfind : ranges.find? (fun r =>
+--       let start := r.endExclusive
+--       let r' := { addr := .ofNat start, size := size }
+--       start ≤ UInt32.size ∧ size.toNat ≤ UInt32.size - start ∧ decide (ranges.Fresh r')) <;> grind
 
 end Sir.Source
